FuseIfte.v
@@ -4,6 +4,7 @@ Require Import PArith.
 Require Import Rustre.Common.
 Require Import Rustre.Minimp.Syntax.
 Require Import Rustre.Minimp.Semantics.
+Require Import Rustre.Minimp.Equiv.
 Require Import Rustre.Dataflow.Syntax.
 Require Import Rustre.Dataflow.Memories.
 Require Import Rustre.Dataflow.IsFree.
@@ -144,14 +145,11 @@ Proof.
 Qed.
 
 Lemma lift_Ifte:
-  forall prog e s1 s2 t1 t2 menv env menv' env',
+  forall e s1 s2 t1 t2,
     (forall x, Is_free_in_exp x e
                -> (~Can_write_in x s1 /\ ~Can_write_in x s2))
-    -> (stmt_eval prog menv env (Comp (Ifte e s1 s2) (Ifte e t1 t2))
-                  (menv', env')
-        <->
-        stmt_eval prog menv env (Ifte e (Comp s1 t1) (Comp s2 t2))
-                  (menv', env')).
+    -> stmt_eval_eq (Comp (Ifte e s1 s2) (Ifte e t1 t2))
+                    (Ifte e (Comp s1 t1) (Comp s2 t2)).
 Proof.
   intros prog e s1 s2 t1 t2 menv env menv' env' Hfw.
   split; intro Hstmt.
@@ -454,5 +452,329 @@ Qed.
    introducing clocking assumptions? The problem is that certain circular
    programs (like the one above) still have a semantics (since x and y
    are effectively always present).
+ *)
+
+Fixpoint ifte_zip s1 s2 : stmt :=
+  match s1, s2 with
+  | Ifte e1 t1 f1, Ifte e2 t2 f2 =>
+      if exp_eqb e1 e2
+      then Ifte e1 (ifte_zip t1 t2) (ifte_zip f1 f2)
+      else Comp s1 s2
+  | Skip, s => s
+  | s,    Skip => s
+  | Comp s1' s2', Ifte _ _ _ => Comp s1' (ifte_zip s2' s2)
+  | s1,   s2 => Comp s1 s2
+  end.
+
+Lemma Can_write_in_ifte_zip:
+  forall s1 s2 x,
+    (Can_write_in x s1 \/ Can_write_in x s2)
+    <-> Can_write_in x (ifte_zip s1 s2).
+Proof.
+  Hint Constructors Can_write_in.
+  induction s1, s2; simpl;
+    repeat progress
+           match goal with
+           | H:Can_write_in _ (Comp _ _) |- _ => inversion H; subst; clear H
+           | H:Can_write_in _ (Ifte _ _ _) |- _ => inversion H; subst; clear H
+           | H:Can_write_in _ Skip |- _ => now inversion H
+           | H:Can_write_in _ _ \/ Can_write_in _ _ |- _ => destruct H
+           | |- context [exp_eqb ?e1 ?e2] =>
+             destruct (exp_eqb e1 e2) eqn:Heq;
+               [apply exp_eqb_eq in Heq; subst|]
+           | |- Can_write_in _ (Ifte _ _ _) =>
+             (apply CWIIfteTrue; apply IHs1_1; now intuition)
+             || (apply CWIIfteFalse; apply IHs1_2; now intuition)
+           | H:Can_write_in _ (ifte_zip _ _) |- _ =>
+             apply IHs1_1 in H || apply IHs1_2 in H
+           | |- Can_write_in _ (Comp _ (ifte_zip _ _)) =>
+             now (apply CWIComp2; apply IHs1_2; intuition)
+           | _ => intuition
+           end.
+Qed.
+
+Lemma Cannot_write_in_ifte_zip:
+  forall s1 s2 x,
+    (~Can_write_in x s1 /\ ~Can_write_in x s2)
+    <-> ~Can_write_in x (ifte_zip s1 s2).
+Proof.
+  intros s1 s2 x.
+  split; intro HH.
+  - intro Hcan; apply Can_write_in_ifte_zip in Hcan; intuition.
+  - split; intro Hcan; apply HH; apply Can_write_in_ifte_zip; intuition.
+Qed.
+
+Lemma ifte_zip_free_write:
+  forall s1 s2,
+    Ifte_free_write s1
+    -> Ifte_free_write s2
+    -> Ifte_free_write (ifte_zip s1 s2).
+Proof.
+  Hint Constructors Ifte_free_write Can_write_in.
+  induction s1, s2;
+    intros Hfree1 Hfree2;
+    inversion_clear Hfree1;
+    simpl;
+    try now intuition.
+  match goal with
+  | |- context [exp_eqb ?e1 ?e2] => destruct (exp_eqb e1 e2) eqn:Heq
+  end; [|intuition].
+  apply exp_eqb_eq in Heq; subst.
+  inversion_clear Hfree2;
+  constructor;
+    repeat progress
+           match goal with
+           | H1:Ifte_free_write ?s1,
+             H2:Ifte_free_write ?s2,
+             Hi:context [Ifte_free_write (ifte_zip _ _)]
+             |- Ifte_free_write (ifte_zip ?s1 ?s2)
+             => apply Hi with (1:=H1) (2:=H2)
+           | |- forall x, Is_free_in_exp x ?e -> _
+             => intros x Hfree
+           | H1:context [Is_free_in_exp _ ?e -> _ /\ _],
+                H2:Is_free_in_exp _ ?e |- _
+             => specialize (H1 _ H2)
+           | |- _ /\ _ => split
+           | |- ~Can_write_in _ (ifte_zip _ _)
+             => apply Cannot_write_in_ifte_zip; intuition
+           | _ => idtac
+           end.
+Qed.
+
+Lemma ifte_zip_Comp':
+  forall s1 s2,
+    Ifte_free_write s1
+    -> (stmt_eval_eq (ifte_zip s1 s2) (Comp s1 s2)).
+Proof.
+  induction s1, s2;
+  try rewrite stmt_eval_eq_Comp_Skip1;
+  try rewrite stmt_eval_eq_Comp_Skip2;
+  try reflexivity;
+  inversion_clear 1;
+  simpl;
+  repeat progress
+         match goal with
+         | |- context [exp_eqb ?e1 ?e2]
+           => destruct (exp_eqb e1 e2) eqn:Heq;
+             [apply exp_eqb_eq in Heq; subst|]
+         | H:Ifte_free_write ?s1,
+             IH:context [stmt_eval_eq (ifte_zip ?s1 _) _]
+           |- context [ifte_zip ?s1 ?s2]
+           => rewrite IH with (1:=H)
+         end;
+  try (rewrite lift_Ifte; [|assumption]);
+  try rewrite Comp_assoc;
+  reflexivity.
+Qed.
+
+Fixpoint ifte_fuse' s1 s2 : stmt :=
+  match s1, s2 with
+  | s1, Comp s2 s3 => ifte_fuse' (ifte_zip s1 s2) s3
+  | s1, s2 => ifte_zip s1 s2
+  end.
+
+Definition ifte_fuse s : stmt :=
+  match s with
+  | Comp s1 (Comp s2 s3) => ifte_fuse' (ifte_zip s1 s2) s3
+  | Comp s1 s2 => ifte_zip s1 s2
+  | _ => s
+  end.
+
+Lemma ifte_fuse'_free_write:
+  forall s2 s1,
+    Ifte_free_write s1
+    -> Ifte_free_write s2
+    -> Ifte_free_write (ifte_fuse' s1 s2).
+Proof.
+  induction s2;
+    try (intros; apply ifte_zip_free_write; assumption).
+  intros s1 Hfree1 Hfree2.
+  inversion_clear Hfree2.
+  apply IHs2_2; [|assumption].
+  apply ifte_zip_free_write; assumption.
+Qed.
+
+(** ifte_eval_eq *)
+
+Require Import Relations.
+Require Import Morphisms.
+Require Import Setoid.
+
+Definition ifte_eval_eq s1 s2: Prop :=
+  stmt_eval_eq s1 s2 /\ (Ifte_free_write s1 /\ Ifte_free_write s2).
+
+(*
+Print relation.
+Check (ifte_eval_eq : relation stmt).
+ *)
+
+Lemma ifte_eval_eq_refl:
+  forall s,
+    Ifte_free_write s
+    -> Proper ifte_eval_eq s.
+Proof.
+  intros s Hfree; unfold Proper, ifte_eval_eq; intuition.
+Qed.
+
+Lemma ifte_eval_eq_trans:
+  transitive stmt ifte_eval_eq.
+Proof.
+  intros s1 s2 s3 Heq1 Heq2.
+  unfold ifte_eval_eq in *.
+  split; [|now intuition].
+  destruct Heq1 as [Heq1 ?].
+  destruct Heq2 as [Heq2 ?].
+  rewrite Heq1, Heq2; reflexivity.
+Qed.
+
+Lemma ifte_eval_eq_sym:
+  symmetric stmt ifte_eval_eq.
+Proof.
+  intros s1 s2 Heq.
+  unfold ifte_eval_eq in *.
+  split; [|now intuition].
+  destruct Heq as [Heq ?].
+  rewrite Heq; reflexivity.
+Qed.
+
+Add Relation stmt (ifte_eval_eq)
+    symmetry proved by ifte_eval_eq_sym
+    transitivity proved by ifte_eval_eq_trans
+  as ifte_eval_equiv.
+
+Lemma subrelation_stmt_ifte_eval_eq:
+  subrelation ifte_eval_eq stmt_eval_eq.
+Proof.
+  intros s1 s2 Heq x menv env menv' env'.
+  now apply Heq.
+Qed.
+
+Lemma ifte_zip_Comp:
+  forall s1 s2,
+    Ifte_free_write s1
+    -> Ifte_free_write s2
+    -> ifte_eval_eq (ifte_zip s1 s2) (Comp s1 s2).
+Proof.
+  intros s1 s2 Hfree1 Hfree2.
+  unfold ifte_eval_eq.
+  split; [|split].
+  - rewrite ifte_zip_Comp' with (1:=Hfree1); reflexivity.
+  - apply ifte_zip_free_write with (1:=Hfree1) (2:=Hfree2).
+  - intuition.
+Qed.
+
+(* TODO: Why don't we get this automatically via the subrelation? *)
+Instance ifte_eval_eq_Proper:
+    Proper (eq ==> eq ==> eq ==> ifte_eval_eq ==> eq ==> iff) stmt_eval.
+Proof.
+  intros prog' prog HR1 menv' menv HR2 env' env HR3 s1 s2 Heq r' r HR4;
+  subst; destruct r as [menv' env'].
+  unfold ifte_eval_eq in Heq.
+  destruct Heq as [Heq ?].
+  rewrite Heq; reflexivity.
+Qed.
+
+Instance ifte_eval_eq_Comp_Proper:
+  Proper (ifte_eval_eq ==> ifte_eval_eq ==> ifte_eval_eq) Comp.
+Proof.
+  Hint Constructors Ifte_free_write.
+  intros s s' Hseq t t' Hteq.
+  unfold ifte_eval_eq in *.
+  destruct Hseq as [Hseq [Hfrees Hfrees']].
+  destruct Hteq as [Hteq [Hfreet Hfreet']].
+  split; [|intuition].
+  rewrite Hseq, Hteq; reflexivity.
+Qed.
+
+Instance ifte_zip_ifte_eval_eq_Proper:
+  Proper (ifte_eval_eq ==> ifte_eval_eq ==> ifte_eval_eq) ifte_zip.
+Proof.
+  intros s s' Hseq t t' Hteq.
+  unfold ifte_eval_eq in *.
+  destruct Hseq as [Hseq [Hfrees Hfrees']].
+  destruct Hteq as [Hteq [Hfreet Hfreet']].
+  split; [|split]; [|apply ifte_zip_free_write with (1:=Hfrees) (2:=Hfreet)
+                    |apply ifte_zip_free_write with (1:=Hfrees') (2:=Hfreet')].
+  rewrite ifte_zip_Comp' with (1:=Hfrees).
+  rewrite ifte_zip_Comp' with (1:=Hfrees').
+  rewrite Hseq, Hteq; reflexivity.
+Qed.
+
+Lemma ifte_fuse'_Comp:
+  forall s2 s1,
+    Ifte_free_write s1
+    -> Ifte_free_write s2
+    -> stmt_eval_eq (ifte_fuse' s1 s2) (Comp s1 s2).
+Proof.
+  Hint Constructors Ifte_free_write.
+  induction s2;
+  intros s1 Hifte1 Hifte2; simpl;
+  try now (rewrite ifte_zip_Comp'; intuition).
+  rewrite Comp_assoc.
+  inversion_clear Hifte2.
+  rewrite IHs2_2;
+    match goal with
+    | H1:Ifte_free_write ?s1,
+      H2:Ifte_free_write ?s2 |- Ifte_free_write (ifte_zip ?s1 ?s2)
+      => apply ifte_zip_free_write with (1:=H1) (2:=H2)
+    | |- Ifte_free_write ?s => assumption
+    | H:Ifte_free_write s2_2 |- _ => pose proof (ifte_eval_eq_refl _ H)
+    end.
+  intros prog menv env menv' env'.
+  rewrite ifte_zip_Comp; [now apply iff_refl|assumption|assumption].
+Qed.
+
+Instance ifte_fuse'_ifte_eval_eq_Proper:
+  Proper (ifte_eval_eq ==> ifte_eval_eq ==> ifte_eval_eq) ifte_fuse'.
+Proof.
+  intros s s' Hseq t t' Hteq.
+  unfold ifte_eval_eq in *.
+  destruct Hseq as [Hseq [Hfrees Hfrees']].
+  destruct Hteq as [Hteq [Hfreet Hfreet']].
+  split; [|split]; [|apply ifte_fuse'_free_write with (1:=Hfrees) (2:=Hfreet)
+                    |apply ifte_fuse'_free_write with (1:=Hfrees') (2:=Hfreet')].
+  repeat rewrite ifte_fuse'_Comp; try assumption.
+  rewrite Hseq, Hteq.
+  reflexivity.
+Qed.
+
+Lemma ifte_fuse_Comp:
+  forall s,
+    Ifte_free_write s
+    -> stmt_eval_eq (ifte_fuse s) s.
+Proof.
+  intros s Hfree prog menv env menv' env'.
+  destruct s; simpl; try reflexivity.
+  inversion_clear Hfree.
+  match goal with
+  | |- _ <-> stmt_eval _ _ _ (Comp ?s1 ?s2) _ =>
+    destruct s2; try (rewrite ifte_zip_Comp;
+                        [reflexivity|assumption|assumption])
+  end.
+  match goal with H: Ifte_free_write (Comp _ _) |- _ => inversion_clear H end.
+  match goal with
+  | H: Ifte_free_write ?s2 |- context [ifte_fuse' _ ?s2]
+    => pose proof (ifte_eval_eq_refl _ H)
+  end.
+  rewrite ifte_zip_Comp; [|assumption|assumption].
+  rewrite Comp_assoc.
+  rewrite ifte_fuse'_Comp; [reflexivity| |assumption].
+  constructor; assumption.
+Qed.
+
+(*
+Eval cbv in (ifte_fuse (Comp (Ifte (Var 1) (Assign 2 (Const (Cint 7))) Skip)
+                             (Comp (Ifte (Var 1) (Assign 4 (Var 2))
+                                         (Assign 4 (State 3)))
+                                   (Comp (Ifte (Var 1) Skip
+                                               (Ifte (Var 2)
+                                                     (AssignSt 3 (Var 2))
+                                                     Skip))
+                                         (Comp (Ifte (Var 1)
+                                                     Skip
+                                                     (Ifte (Var 2)
+                                                           (AssignSt 3 (Var 4))
+                                                           Skip)) Skip))))).
 *)
+
 
