Minimp.v
@@ -1,2 +1,3 @@
 Require Export Minimp.Syntax.
 Require Export Minimp.Semantics.
+Require Export Minimp.Equiv.
